WIP rappend

lambda2Gmu/.Makefile.d
@@ -28,9 +28,9 @@ Prelude.vos Prelude.vok Prelude.required_vos: Prelude.v Zip.vos Definitions.vos 
 Preservation.vo Preservation.glob Preservation.v.beautified Preservation.required_vo: Preservation.v Prelude.vo Infrastructure.vo Regularity.vo Equations.vo
 Preservation.vio: Preservation.v Prelude.vio Infrastructure.vio Regularity.vio Equations.vio
 Preservation.vos Preservation.vok Preservation.required_vos: Preservation.v Prelude.vos Infrastructure.vos Regularity.vos Equations.vos
-Progress.vo Progress.glob Progress.v.beautified Progress.required_vo: Progress.v Prelude.vo Infrastructure.vo Regularity.vo CanonicalForms.vo
-Progress.vio: Progress.v Prelude.vio Infrastructure.vio Regularity.vio CanonicalForms.vio
-Progress.vos Progress.vok Progress.required_vos: Progress.v Prelude.vos Infrastructure.vos Regularity.vos CanonicalForms.vos
+Progress.vo Progress.glob Progress.v.beautified Progress.required_vo: Progress.v Prelude.vo Infrastructure.vo Regularity.vo CanonicalForms.vo Equations.vo
+Progress.vio: Progress.v Prelude.vio Infrastructure.vio Regularity.vio CanonicalForms.vio Equations.vio
+Progress.vos Progress.vok Progress.required_vos: Progress.v Prelude.vos Infrastructure.vos Regularity.vos CanonicalForms.vos Equations.vos
 Regularity.vo Regularity.glob Regularity.v.beautified Regularity.required_vo: Regularity.v Prelude.vo Infrastructure.vo Equations.vo
 Regularity.vio: Regularity.v Prelude.vio Infrastructure.vio Equations.vio
 Regularity.vos Regularity.vok Regularity.required_vos: Regularity.v Prelude.vos Infrastructure.vos Equations.vos
